@prefix mbco: <https://batcat.info/semantics/core#> . 

@prefix dc: <http://purl.org/dc/elements/1.1/> .
@prefix dcterms: <http://purl.org/dc/terms/> .  
#@prefix mod: <https://w3id.org/mod#> .
@prefix owl: <http://www.w3.org/2002/07/owl#> .
@prefix rdf: <http://www.w3.org/1999/02/22-rdf-syntax-ns#> .  
@prefix rdfs: <http://www.w3.org/2000/01/rdf-schema#> .
@prefix skos: <http://www.w3.org/2004/02/skos/core#> .
@prefix xs: <http://www.w3.org/2001/XMLSchema#> .

<https://batcat.info/semantics/core/optimization#> a owl:Ontology .

<https://batcat.info/semantics/core/optimization#> dcterms:title "BatCAT core ontologies: module for Optimization, decision support and design"^^xs:string ;
  owl:versionInfo "version 0.1.3"^^xs:string ;
  dcterms:modified "2025-05-12"^^xs:string ;
  owl:imports <https://batcat.info/semantics/core#> ;
  dcterms:creator "Silvia Chiacchiera (ORCID 0000-0003-0422-7870)"^^xs:string ;
  dcterms:contributor "Martin T. Horsch (ORCID 0000-0002-9464-6739)"^^xs:string ;
  dcterms:contributor "Gerhard Goldbeck (ORCID 0000-0002-4181-2852)"^^xs:string ;
  dcterms:contributor "Fadi Al Machot (ORCID 0000-0002-1239-9261)"^^xs:string ;
  dcterms:contributor "Martin Petit (ORCID 0000-0002-4226-6689)"^^xs:string ;
  dcterms:contributor "Martin Gebser (ORCID 0000-0002-8010-4752)"^^xs:string ;
  dcterms:contributor "Mohamed El Bahnasawi (ORCID 0000-0001-9600-3182)"^^xs:string ;  
  dcterms:contributor "Noel Vizcaino"^^xs:string ;
  dcterms:contributor "Ilian T. Todorov (ORCID 0000-0001-7275-1784)"^^xs:string ;
  dcterms:license "https://www.gnu.org/licenses/lgpl-3.0.en.html"^^xs:anyURI ;
  dcterms:description """The aim of BatCAT core ontologies is covering all needed aspects of the battery domain,
with a focus on Industry 5.0 cell manufacturing and addressing BatCAT use-cases."""^^xs:string ;
#  dcterms:bibliographicCitation ""^^xs:string ;
  rdfs:comment """The authors acknowledge funding from the European Union's Horizon Europe research and
innovation programme under grant agreement no. 101137725, Battery Cell Assembly Twin (BatCAT)."""^^xs:string .

### Classes ###

mbco:problem a owl:Class ;
    rdfs:label "Problem" ; # TODO: do we need this class? Or does it make the hierarchy too deep?
    rdfs:subClassOf mbco:statement .

mbco:solution a owl:Class ;
    rdfs:label "Solution" ;
    rdfs:comment "Answer addressing a problem. It should contain a quantification of error and confidence."^^xs:string ;
    rdfs:subClassOf mbco:statement .

mbco:solution rdfs:subClassOf [a owl:Restriction ;
                   owl:onProperty mbco:has_confidence ;
                   owl:someValuesFrom mbco:coarse_amount_level] .

mbco:optimization_problem a owl:Class ;
    rdfs:label "Optimization problem" ;
    rdfs:subClassOf mbco:problem .

mbco:optimization_method a owl:Class ; # TOSEE: or are they "problem solving methods???"
    rdfs:label "Optimization method" ;
    rdfs:subClassOf mbco:method ;
    a owl:DeprecatedClass .

mbco:answer_set_programming a owl:Class ;
    rdfs:label "Answer Set Programming (ASP)" ;
    rdfs:subClassOf mbco:optimization_method ; # correct??? It is a "logic programming method/paradigm"
    rdfs:comment "A logic programming paradigm, tailored to search problems. (See Wikipedia)"^^xs:string .

mbco:multi_criteria_optimization a owl:Class ;
    rdfs:label "Multi Criteria Optimization (MCO)" ;
    rdfs:subClassOf mbco:optimization_method ;
    rdfs:comment "Mathematical optimization problem, where multiple objective functions (criteria) are simultaneuosly optimized. (See Wikipedia)"^^xs:string .

mbco:mathematical_role a owl:Class ;
    rdfs:label "Mathematical role" ;
    rdfs:subClassOf mbco:role .

mbco:variable a owl:Class ;
    rdfs:label "Variable" ;
    owl:disjointUnionOf (mbco:discrete_variable mbco:continuum_variable) ;
    rdfs:subClassOf mbco:mathematical_role .		

mbco:discrete_variable a owl:Class ;
    rdfs:label "Discrete variable" ;
    rdfs:subClassOf mbco:variable .

mbco:continuum_variable a owl:Class ;
    rdfs:label "Continuum variable" ;
    rdfs:subClassOf mbco:variable .

mbco:target a owl:Class ;
    rdfs:label "Target" ;
    rdfs:subClassOf mbco:mathematical_role ;
    rdfs:comment "In an optimization problem, a property which has to be attained exactly or approximatively by the solution."^^xs:string .

mbco:goal a owl:Class ;
    rdfs:label "Goal" ;
    rdfs:altLabel "Exact target" ;
    rdfs:subClassOf mbco:target ;
    rdfs:comment "In an optimization problem, a property which must be attained exactly by a solution."^^xs:string ;
    rdfs:comment "In an optimization problem, an exact target."^^xs:string .

mbco:constraint a owl:Class ;
    rdfs:label "Constraint" ;
    rdfs:subClassOf mbco:statement ;		    
    owl:disjointUnionOf (mbco:qualitative_constraint mbco:quantitative_constraint) .

mbco:qualitative_constraint a owl:Class ;
    rdfs:label "Qualitative constraint" ;
    rdfs:comment "Examples of qualtitative constraints are: step X follows (directly) step Y; step X requires participant Y; step X requires input Y; physical location constraint."^^xs:string .

mbco:quantitative_constraint a owl:Class ;
    rdfs:label "Quantitative constraint" ;
    rdfs:comment "Examples of quantitative constraints are equalities (e.g., the sum of some variables is constant) and inequalitites (variable X > value X0)."^^xs:string .

mbco:optimization_problem  # TOSEE: Do these restrictions apply to all problems?
	rdfs:subClassOf [a owl:Restriction ;
                   owl:onProperty mbco:has_part ;
                   owl:someValuesFrom mbco:variable] ;
	rdfs:subClassOf [a owl:Restriction ;
                   owl:onProperty mbco:has_part ;
                   owl:someValuesFrom mbco:target] ;
	rdfs:subClassOf [a owl:Restriction ;
                   owl:onProperty mbco:has_part ;
                   owl:someValuesFrom mbco:constraint] ;
	rdfs:subClassOf [a owl:Restriction ;
                   owl:onProperty mbco:has_part ;
                   owl:someValuesFrom mbco:goal] ;
	rdfs:subClassOf [a owl:Restriction ;
                   owl:onProperty mbco:has_part ;
                   owl:someValuesFrom mbco:initial_status] .  
		  
mbco:coarse_amount_level a owl:Class ; # TOSEE: create a "quantifier" class? TOSEE: move this to "higher" module?
    rdfs:label "(Coarse) Amount level" ;
    owl:oneOf (mbco:LOW mbco:MEDIUM mbco:HIGH) ;
    rdfs:subClassOf mbco:data . # ok?

mbco:initial_status a owl:Class ; 
    rdfs:label "Initial status" ;
    rdfs:subClassOf mbco:status ;
    rdfs:comment "Status of an object/system right at the start of a given process. E.g., before an optimization is done"^^xs:string .    

mbco:final_status a owl:Class ; 
    rdfs:label "Final status" ;
    rdfs:subClassOf mbco:status ;
    rdfs:comment "Status of an object/system right at the end of a given process. E.g., after an optimization is done"^^xs:string .    

# Examples of general logic-based problems/activity. TOSEE: Are these really optimization problems??? Problems? Logic-based problems? Are these activities? goals? Tasks?
# Taken from CQ_CRO_8

mbco:logic_based_problem a owl:Class ;
    rdfs:label "Logic-based problem" ;
    rdfs:subClassOf mbco:problem .

mbco:numerical_problem a owl:Class ;
    rdfs:label "Numerical problem" ;
    rdfs:subClassOf mbco:problem .

mbco:scheduling a owl:Class ;
    rdfs:label "Scheduling" ;
    rdfs:comment "Scheduling (e.g., of maintenance)"^^xs:string ;
    rdfs:subClassOf mbco:logic_based_problem .

mbco:resource_allocation a owl:Class ;
    rdfs:label "Resource allocation" ;
    rdfs:comment "Allocation of resources (e.g., machines/humans for tasks)"^^xs:string ;
    rdfs:subClassOf mbco:logic_based_problem .

mbco:compatibility_check a owl:Class ;
    rdfs:label "Compatibility check" ;
    rdfs:comment "Compatibility checks (e.g., between materials)"^^xs:string ;
    rdfs:subClassOf mbco:logic_based_problem .

mbco:compliance_validation a owl:Class ;
    rdfs:label "Compliance validation" ;
    rdfs:comment "Compliance validation (e.g., of a process with regulation)"^^xs:string ;
    rdfs:subClassOf mbco:logic_based_problem .

mbco:process_design a owl:Class ;
    rdfs:label "Process design" ;
    rdfs:comment "Process design (e.g., simulation, experiment)"^^xs:string ;
    rdfs:subClassOf mbco:logic_based_problem ;
    rdfs:subClassOf mbco:numerical_problem . # right?

mbco:process_sequence_validation a owl:Class ;
    rdfs:label "Process sequence validation" ;
    rdfs:comment "Process sequence validation (e.g., that the ordering of sub-processes does not break dependencies)"^^xs:string ;
    rdfs:subClassOf mbco:logic_based_problem .

mbco:model_parametrization_process a owl:Class ; # this is for MCO
    rdfs:label "Model parametrization process" ;
    rdfs:comment "Determining the numerical values of the parameters as those that best reproduce certain properties. "^^xs:string ;
    rdfs:comment "Not to be confused with the resulting model parameterization (a set of parameters)."^^xs:string ;
    rdfs:subClassOf mbco:numerical_problem .

### Object Properties ###

mbco:has_cost_level a owl:ObjectProperty ; # TOSEE: express it differently? Issue is: if we use more general verbs, the statements are more complex.
    rdfs:comment "Points to the cost of an entity, in the broad sense. It could be monetary cost, computational cost, etc."^^xs:string ;
    rdfs:range mbco:coarse_amount_level .

mbco:has_precision_level a owl:ObjectProperty ;  # TOSEE: same as for has_cost_level
    rdfs:range mbco:coarse_amount_level .

mbco:has_confidence_level a owl:ObjectProperty ;
    rdfs:comment "Points to the confidence in the correctness of a statement, and is generated by the same source."^^xs:string ;
    rdfs:range mbco:coarse_amount_level ;
    rdfs:domain mbco:statement .

### Datatype Properties ###

### Other tentative properties still under consideration ...

# mbco:has_quantifier
# mbco:has_confidence
# mbco:has_error
# mbco:has_assumption
# mbco:has_variable
# mbco:has_target
# mbco:has_constraint 
#
# Other: design_parameters, operating conditions, cost, KPI

####################################################################################
# EXAMPLES below: Put here temporarily only, just for simplicity
####################################################################################

@prefix ex: <https://batcat.info/semantics/example#> .

ex:GITT_TEST a mbco:method ;
    mbco:has_output ex:DIFFUSION_COEFFICIENT ;
    mbco:has_output ex:ACTIVE_MATERIAL_POTENTIALS ;
    mbco:has_participant ex:POTENTIOSTAT ;
    mbco:has_participant [a mbco:sample] ;
    mbco:has_participant [a mbco:agent] ;
    mbco:has_cost_level mbco:HIGH ;
    mbco:has_precision_level mbco:HIGH .       

ex:DISSIPATIVE_PARTICLE_DYNAMICS a mbco:method ;
    mbco:has_input ex:DPD_MODEL_PARAMETRIZATION_1 ;
    mbco:has_output ex:DIFFUSION_COEFFICIENT ;
    mbco:has_participant [a mbco:computational_device] ;
    mbco:has_participant [a mbco:software] ; # E.g., license access needed
    mbco:has_cost_level mbco:MEDIUM ;
    mbco:has_precision_level mbco:LOW .       
#    mbco:has_property ex:DPD_COST, ex:DPD_PRECISION .

ex:DPD_DATA_ANALYSIS a mbco:process ;
    mbco:has_participant [a mbco:agent] .		   

ex:DPD_SIMULATION_SETTING_UP a mbco:process ;
    mbco:has_participant [a mbco:agent] .

ex:EXPERIMENT_SETTING_UP a mbco:process ;
    mbco:has_participant [a mbco:agent] .		   

ex:RESOURCE_ALLOCATION_EXAMPLE_PROBLEM
    a mbco:logic_based_problem ;
    a mbco:optimization_problem ;
    rdfs:comment "An example about running simulations"^^xs:string ;
    mbco:has_part ex:GOAL_1 ;
    mbco:has_part ex:TARGET_2 ;
    mbco:has_part ex:CONSTRAINT_1 ;
    mbco:has_part ex:CONSTRAINT_2 ;
    mbco:has_part ex:CONSTRAINT_3 ;
    mbco:has_part ex:INITIAL_STATUS_1 .

ex:GOAL_1 a mbco:goal ;
   rdfs:comment "Allocate human and computational devices to run 2 DPD simulations, respecting the ordering of steps."^^xs:string .

ex:INITIAL_STATUS_1 a mbco:initial_status ;
   rdfs:comment "Human and computational devices are available and operational. Needed software is installed"^^xs:string .

ex:TARGET_2 a mbco:target ;
   rdfs:comment "Maximize usage of resources (minimize their idle time)."^^xs:string .

ex:CONSTRAINT_1 a mbco:quantitative_constraint ;
    rdfs:comment "There is only one available agent"^^xs:string .

ex:CONSTRAINT_2 a mbco:quantitative_constraint ;
    rdfs:comment "There are two available computational devices"^^xs:string .

ex:CONSTRAINT_3 a mbco:qualitative_constraint ;
    rdfs:comment "A computational method must be used"^^xs:string .

ex:DPD_SIMULATION_RUN 
    mbco:uses_method ex:DISSIPATIVE_PARTICLE_DYNAMICS ;
    mbco:followsdirectly ex:DPD_SIMULATION_SETTING_UP .

ex:DPD_DATA_ANALYSIS mbco:followsdirectly ex:DPD_SIMULATION_RUN .

ex:COMPARISON_EXAMPLE_PROBLEM
    a mbco:logic_based_problem ;
    a mbco:optimization_problem ;
    rdfs:comment "An example about comparing simulations or experiments"^^xs:string ;
    mbco:has_part ex:GOAL_2 ;
    mbco:has_part ex:TARGET_1 .

ex:GOAL_2 a mbco:qualitative_constraint ;
    rdfs:comment "Evaluate the diffusion coefficient of a substance"^^xs:string .

ex:TARGET_1 a mbco:target ;
   rdfs:comment "Maximize precision and minimize cost"^^xs:string .

ex:SOLUTION_COMPARISON a mbco:solution ;
   mbco:answers ex:COMPARISON_EXAMPLE_PROBLEM ;
   mbco:uses_method [a mbco:answer_set_programming] .

ex:SOLUTION_RESOURCE_ALLOCATION a mbco:solution ;
   mbco:answers ex:RESOURCE_ALLOCATION_EXAMPLE_PROBLEM ;
   mbco:uses_method [a mbco:answer_set_programming] .

####################################################################################
# See also:
# inequality # EMMO - Math module (under "disciplines") 
# equality # EMMO - Math module (under "disciplines") - it has "equation"
# variable from VOV could be used. Also present in EMMO "math"
