@prefix mbco: <https://batcat.info/semantics/core#> . 

@prefix dc: <http://purl.org/dc/elements/1.1/> .
@prefix dcterms: <http://purl.org/dc/terms/> .  
#@prefix mod: <https://w3id.org/mod#> .
@prefix owl: <http://www.w3.org/2002/07/owl#> .
@prefix rdf: <http://www.w3.org/1999/02/22-rdf-syntax-ns#> .  
@prefix rdfs: <http://www.w3.org/2000/01/rdf-schema#> .
@prefix skos: <http://www.w3.org/2004/02/skos/core#> .
@prefix xs: <http://www.w3.org/2001/XMLSchema#> .

<https://batcat.info/semantics/core/twinning#> a owl:Ontology .

<https://batcat.info/semantics/core/twinning#> dcterms:title "BatCAT core ontologies: module for (Digital) Twinning"^^xs:string ;
  owl:versionInfo "version 0.0.3"^^xs:string ;
  dcterms:modified "2025-12-03"^^xs:string ;
  owl:imports <https://batcat.info/semantics/core#> ;
  dcterms:creator "Silvia Chiacchiera (ORCID 0000-0003-0422-7870)"^^xs:string ;
  dcterms:contributor "Martin T. Horsch (ORCID 0000-0002-9464-6739)"^^xs:string ;
  dcterms:contributor "Gerhard Goldbeck (ORCID 0000-0002-4181-2852)"^^xs:string ;
  dcterms:contributor "Fadi Al Machot (ORCID 0000-0002-1239-9261)"^^xs:string ;
  dcterms:contributor "Noel Vizcaino (ORCID 0000-0001-7608-9484)"^^xs:string ;
  dcterms:contributor "Ilian T. Todorov (ORCID 0000-0001-7275-1784)"^^xs:string ;
  dcterms:license "https://www.gnu.org/licenses/lgpl-3.0.en.html"^^xs:anyURI ;
  dcterms:description """The aim of BatCAT core ontologies is covering all needed aspects of the battery domain,
with a focus on Industry 5.0 cell manufacturing and addressing BatCAT use-cases."""^^xs:string ;
#  dcterms:bibliographicCitation ""^^xs:string ;
  rdfs:comment """The authors acknowledge funding from the European Union's Horizon Europe research and
innovation programme under grant agreement no. 101137725, Battery Cell Assembly Twin (BatCAT)."""^^xs:string .

### Classes ###

# CAVEAT: Duplicated here from modelling.ttl for convenience
mbco:digital_twinning a owl:Class ; 
    rdfs:label "Digital twinning" ;
    rdfs:subClassOf mbco:computational_modelling_method .
mbco:computational_modelling_method rdfs:subClassOf mbco:method .    
# end of duplication

mbco:digital_twin_model a owl:Class ; 
    rdfs:label "Digital twin model" ;
    rdfs:subClassOf mbco:data ; # TOSEE: define a model class?
    rdfs:subClassOf [a owl:Restriction ;
                   owl:onProperty mbco:represents ;
                   owl:someValuesFrom owl:Thing] ;
    rdfs:subClassOf [a owl:Restriction ;
                   owl:onProperty mbco:has_action_type ;
                   owl:someValuesFrom mbco:digital_twin_action] ;
    rdfs:subClassOf [a owl:Restriction ;
                   owl:onProperty mbco:has_synchronization_rate ;
                   owl:someValuesFrom xs:decimal] .

mbco:digital_twin_action a owl:Class ;
    rdfs:label "Digital twin action" ;
    owl:oneOf (mbco:VISUALIZE mbco:MONITOR mbco:PREDICT mbco:RECOMMEND) ;
    rdfs:comment """Based on an extract of application-related terms from ISO/IEC 30173:2023, 
    with an addition inspired by Barros et al. 2021, 'Requirements for an Ontology of Digital Twins'."""^^xs:string ;
    rdfs:subClassOf mbco:process .

mbco:generality_level a owl:Class ; 
    owl:oneOf (mbco:UNIVERSAL mbco:TYPE mbco:INDIVIDUAL) ;
    rdfs:comment "Inspired by Barros et al. 2021, 'Requirements for an Ontology of Digital Twins'. Note: There a fourth level is present."^^xs:string ;
    rdfs:subClassOf mbco:annotation .

mbco:UNIVERSAL rdfs:comment "Encompassing, e.g. for a very generic entity or process."^^xs:string .
mbco:TYPE rdfs:comment "E.g., a car. Inspired by Barros et al. 2021, 'Requirements for an Ontology of Digital Twins'."^^xs:string .
mbco:INDIVIDUAL rdfs:comment "E.g., John's car. Inspired by Barros et al. 2021, 'Requirements for an Ontology of Digital Twins'."^^xs:string .

### Object Properties ###

mbco:represents a owl:ObjectProperty ;
    rdfs:label "represents" ;
    rdfs:range [owl:unionOf (mbco:physical_object mbco:process)] .

#mbco:has_action_type a owl:ObjectProperty ; # now defined in modelling.ttl
#    rdfs:label "has action type" .
#    rdfs:range mbco:digital_twin_action .

mbco:has_generality_level a owl:ObjectProperty ;
    rdfs:label "has generality level" ;
    rdfs:range mbco:generality_level .
    
### Datatype Properties ###

mbco:has_synchronization_rate a owl:DatatypeProperty ;
    rdfs:label "has synchronization rate" ;
    rdfs:comment """(Average) Rate (in 1/seconds) at which communication (in either direction) between 
    the digital entity and its target entity happens"""^^xs:string .

####################################################################################
# EXAMPLES below: Put here temporarily only, just for simplicity
####################################################################################

@prefix ex: <https://batcat.info/semantics/example#> .

ex:DT_LIB_CELL_C032 a mbco:digital_twin_model ;
    mbco:has_generality_level mbco:TYPE ;
    rdfs:comment "Digital twin of a LiB cell of type C032"^^xs:string .

ex:DT_LIB_CELL_C032_PID123456 a mbco:digital_twin_model ;
    mbco:has_generality_level mbco:INDIVIDUAL ;
    mbco:has_synchronization_rate 1.0 ;
    rdfs:comment "Digital twin of a specific LiB cell of type C032, identified by its PID"^^xs:string .

####################################################################################
